Use notation in proof-facing definitions

Denotation/theories/TypeDenote.v
@@ -6,16 +6,44 @@ Section TypeDenote.
 
 Definition ty_guard_formula
     (Σ : lty_env) (τ : context_ty) (e : tm) : FormulaT :=
-  FAnd (context_ty_wf_formula Σ τ)
-    (FAnd (basic_world_formula Σ)
-      (FAnd (expr_basic_typing_formula Σ e (erase_ty τ))
-            (expr_total_formula e))).
+  (FWfTy[Σ; τ] ∧
+    (FWorld[Σ] ∧
+      (FHasType[Σ ⊢ e ⋮ (⌊τ⌋)%cty] ∧ FTotal[e])))%formula.
 
 Definition ty_static_guard_formula
     (Σ : lty_env) (τ : context_ty) (e : tm) : FormulaT :=
-  FAnd (context_ty_wf_formula Σ τ)
-    (FAnd (basic_world_formula Σ)
-      (expr_basic_typing_formula Σ e (erase_ty τ))).
+  (FWfTy[Σ; τ] ∧
+    (FWorld[Σ] ∧ FHasType[Σ ⊢ e ⋮ (⌊τ⌋)%cty]))%formula.
+
+Notation "'guard[' Σ ']' τ" :=
+  (ty_guard_formula Σ τ)
+  (at level 20, Σ at level 200, τ at level 200,
+   format "guard[ Σ ]  τ").
+
+Notation "'guard[' Σ ']' τ e" :=
+  (ty_guard_formula Σ τ e)
+  (at level 20, Σ at level 200, τ at level 200, e at level 20,
+   format "guard[ Σ ]  τ  e").
+
+Notation "'guard[' Σ ';' τ ';' e ']'" :=
+  (ty_guard_formula Σ τ e)
+  (at level 20, Σ at level 200, τ at level 200, e at level 200,
+   format "guard[ Σ ;  τ ;  e ]").
+
+Notation "'static_guard[' Σ ']' τ" :=
+  (ty_static_guard_formula Σ τ)
+  (at level 20, Σ at level 200, τ at level 200,
+   format "static_guard[ Σ ]  τ").
+
+Notation "'static_guard[' Σ ']' τ e" :=
+  (ty_static_guard_formula Σ τ e)
+  (at level 20, Σ at level 200, τ at level 200, e at level 20,
+   format "static_guard[ Σ ]  τ  e").
+
+Notation "'static_guard[' Σ ';' τ ';' e ']'" :=
+  (ty_static_guard_formula Σ τ e)
+  (at level 20, Σ at level 200, τ at level 200, e at level 200,
+   format "static_guard[ Σ ;  τ ;  e ]").
 
 Lemma fiberwise_joinable_on_ty_static_guard_formula X Σ τ e :
   fiberwise_joinable_on X (ty_static_guard_formula Σ τ e).
@@ -50,16 +78,13 @@ Lemma fiberwise_joinable_ty_guard_formula Σ τ e :
 Proof. intros X. apply fiberwise_joinable_on_ty_guard_formula. Qed.
 
 Definition result_basic_typing_formula (b : base_ty) : FormulaT :=
-  expr_basic_typing_formula
-    (typed_lty_env_bind ∅ (TBase b))
-    (tret (vbvar 0))
-    (TBase b).
+  FHasType[(∅ ▷ TBase b)%lvar ⊢ (ret # 0)%core ⋮ TBase b].
 
 Definition over_result_body (b : base_ty) (φ : type_qualifier) : FormulaT :=
-  FOver (FAnd (FAtom φ) (result_basic_typing_formula b)).
+  (over (@atom φ ∧ result_basic_typing_formula b))%formula.
 
 Definition under_result_body (b : base_ty) (φ : type_qualifier) : FormulaT :=
-  FUnder (FAnd (FAtom φ) (result_basic_typing_formula b)).
+  (under (@atom φ ∧ result_basic_typing_formula b))%formula.
 
 Lemma formula_fv_result_basic_typing_formula b :
   formula_fv (result_basic_typing_formula b) = ∅.
@@ -76,96 +101,71 @@ Definition arrow_value_denote_gas_with
     (denote : nat -> lty_env -> context_ty -> tm -> FormulaT)
     (gas : nat) (Σ : lty_env) (τx τr : context_ty) (ef : tm) :
     FormulaT :=
-  let Σx := typed_lty_env_bind Σ (erase_ty τx) in
-  FForall
-    (FImpl
-      (denote gas Σx
-        (cty_shift 0 τx) (tret (vbvar 0)))
-      (denote gas Σx τr
-        (tapp_tm (tm_shift 0 ef) (vbvar 0)))).
+  let Σx := (Σ ▷ (⌊τx⌋)%cty)%lvar in
+  (∀.
+    denote gas Σx (τx ↑)%cty (ret # 0)%core →
+    denote gas Σx τr ((ef ↑)%core ·ₜ # 0))%formula.
 
 Definition wand_value_denote_gas_with
     (denote : nat -> lty_env -> context_ty -> tm -> FormulaT)
     (gas : nat) (Σ : lty_env) (τx τr : context_ty) (ef : tm) :
     FormulaT :=
-  let Σx := typed_lty_env_bind Σ (erase_ty τx) in
-  FBWand 1
-    (denote gas Σx
-      (cty_shift 0 τx) (tret (vbvar 0)))
-    (denote gas Σx τr
-      (tapp_tm (tm_shift 0 ef) (vbvar 0))).
+  let Σx := (Σ ▷ (⌊τx⌋)%cty)%lvar in
+  (denote gas Σx (τx ↑)%cty (ret # 0)%core -∗[1]
+   denote gas Σx τr ((ef ↑)%core ·ₜ # 0))%formula.
 
 Fixpoint ty_denote_gas
     (gas : nat) (Σ : lty_env) (τ : context_ty) (e : tm)
     {struct gas} : FormulaT :=
   let Σg := relevant_env Σ τ e in
-  FAnd
-    (ty_guard_formula Σg τ e)
+  (guard[Σg; τ; e] ∧
     (match gas with
-    | 0 => FTrue
+    | 0 => ⊤
     | S gas' =>
       match τ with
       | CTOver b φ =>
-          FForall
-            (FImpl
-              (expr_result_formula_at (lvars_shift_from 0 (dom Σg))
-                (tm_shift 0 e) (LVBound 0))
-              (FFibVars (qual_vars φ ∖ {[LVBound 0]})
-                (over_result_body b φ)))
+          (∀.
+            FResult[(⇑ₗ (dom Σg))%lvar ⊢ (e ↑)%core ⇓ #ₗ 0] →
+            fib (qual_vars φ ∖ {[LVBound 0]}) |>
+              over (@atom φ ∧
+                FHasType[(∅ ▷ TBase b)%lvar ⊢ (ret # 0)%core ⋮ TBase b]))%formula
       | CTUnder b φ =>
-          FForall
-            (FImpl
-              (expr_result_formula_at (lvars_shift_from 0 (dom Σg))
-                (tm_shift 0 e) (LVBound 0))
-              (FFibVars (qual_vars φ ∖ {[LVBound 0]})
-                (under_result_body b φ)))
+          (∀.
+            FResult[(⇑ₗ (dom Σg))%lvar ⊢ (e ↑)%core ⇓ #ₗ 0] →
+            fib (qual_vars φ ∖ {[LVBound 0]}) |>
+              under (@atom φ ∧
+                FHasType[(∅ ▷ TBase b)%lvar ⊢ (ret # 0)%core ⋮ TBase b]))%formula
       | CTInter τ1 τ2 =>
-          FAnd
-            (ty_denote_gas gas' Σ τ1 e)
-            (ty_denote_gas gas' Σ τ2 e)
+          (ty_denote_gas gas' Σ τ1 e ∧
+           ty_denote_gas gas' Σ τ2 e)%formula
       | CTUnion τ1 τ2 =>
-          FOr
-            (ty_denote_gas gas' Σ τ1 e)
-            (ty_denote_gas gas' Σ τ2 e)
+          (ty_denote_gas gas' Σ τ1 e ∨
+           ty_denote_gas gas' Σ τ2 e)%formula
       | CTSum τ1 τ2 =>
-          let Σr := typed_lty_env_bind Σg (erase_ty τ1) in
-          FForall
-            (FImpl
-              (expr_result_formula_at (lvars_shift_from 0 (dom Σg))
-                (tm_shift 0 e) (LVBound 0))
-              (FPlus
-                (ty_denote_gas gas' Σr
-                  (cty_shift 0 τ1) (tret (vbvar 0)))
-                (ty_denote_gas gas' Σr
-                  (cty_shift 0 τ2) (tret (vbvar 0)))))
+          let Σr := (Σg ▷ (⌊τ1⌋)%cty)%lvar in
+          (∀.
+            FResult[(⇑ₗ (dom Σg))%lvar ⊢ (e ↑)%core ⇓ #ₗ 0] →
+            ty_denote_gas gas' Σr (τ1 ↑)%cty (ret # 0)%core ⊕
+            ty_denote_gas gas' Σr (τ2 ↑)%cty (ret # 0)%core)%formula
       | CTArrow τx τr =>
-          let Σf := typed_lty_env_bind Σg (erase_ty (CTArrow τx τr)) in
-          FForall
-            (FImpl
-              (expr_result_formula_at (lvars_shift_from 0 (dom Σg))
-                (tm_shift 0 e) (LVBound 0))
-              (arrow_value_denote_gas_with ty_denote_gas gas' Σf
-                (cty_shift 0 τx) (cty_shift 1 τr)
-                (tret (vbvar 0))))
+          let Σf := (Σg ▷ (⌊(τx → τr)%cty⌋)%cty)%lvar in
+          (∀.
+            FResult[(⇑ₗ (dom Σg))%lvar ⊢ (e ↑)%core ⇓ #ₗ 0] →
+            arrow_value_denote_gas_with ty_denote_gas gas' Σf
+              (τx ↑)%cty (↑{1} τr)%cty (ret # 0)%core)%formula
       | CTWand τx τr =>
-          let Σf := typed_lty_env_bind Σg (erase_ty (CTWand τx τr)) in
-          FForall
-            (FImpl
-              (expr_result_formula_at (lvars_shift_from 0 (dom Σg))
-                (tm_shift 0 e) (LVBound 0))
-              (wand_value_denote_gas_with ty_denote_gas gas' Σf
-                (cty_shift 0 τx) (cty_shift 1 τr)
-                (tret (vbvar 0))))
-      | CTPersist τ1=>
-          let Σr := typed_lty_env_bind Σg (erase_ty (CTPersist τ1)) in
-          FForall
-            (FImpl
-              (expr_result_formula_at (lvars_shift_from 0 (dom Σg))
-                (tm_shift 0 e) (LVBound 0))
-              (FPersist (ty_denote_gas gas' Σr
-                    (cty_shift 0 τ1) (tret (vbvar 0)))))
+          let Σf := (Σg ▷ (⌊(τx -∗ τr)%cty⌋)%cty)%lvar in
+          (∀.
+            FResult[(⇑ₗ (dom Σg))%lvar ⊢ (e ↑)%core ⇓ #ₗ 0] →
+            wand_value_denote_gas_with ty_denote_gas gas' Σf
+              (τx ↑)%cty (↑{1} τr)%cty (ret # 0)%core)%formula
+      | CTPersist τ1 =>
+          let Σr := (Σg ▷ (⌊(□ τ1)%cty⌋)%cty)%lvar in
+          (∀.
+            FResult[(⇑ₗ (dom Σg))%lvar ⊢ (e ↑)%core ⇓ #ₗ 0] →
+            □ (ty_denote_gas gas' Σr (τ1 ↑)%cty (ret # 0)%core))%formula
     end
-    end).
+    end))%formula.
 
 Definition arrow_value_denote_gas :=
   arrow_value_denote_gas_with ty_denote_gas.
@@ -198,6 +198,11 @@ Notation "'⟦ty' τ '⟧[' Δ ']' e" :=
   (at level 20, τ at level 200, Δ at level 200, e at level 20,
    only parsing).
 
+Notation "'TyDenote[' Δ ';' τ ';' e ']'" :=
+  (ty_denote Δ τ e)
+  (at level 20, Δ at level 200, τ at level 200, e at level 200,
+   format "TyDenote[ Δ ;  τ ;  e ]").
+
 Notation "'⟦ty⟧[' Σ ',' gas ']' τ" :=
   (ty_denote_gas gas Σ τ)
   (at level 20, Σ at level 200, gas at level 9, τ at level 200,
@@ -219,24 +224,9 @@ Notation "'⟦ty⟧[' Δ ']' τ e" :=
   (at level 20, Δ at level 200, τ at level 200, e at level 20,
    format "⟦ty⟧[ Δ ]  τ  e").
 
-Notation "'guard[' Σ ']' τ" :=
-  (ty_guard_formula Σ τ)
-  (at level 20, Σ at level 200, τ at level 200,
-   format "guard[ Σ ]  τ").
-
-Notation "'guard[' Σ ']' τ e" :=
-  (ty_guard_formula Σ τ e)
-  (at level 20, Σ at level 200, τ at level 200, e at level 20,
-   format "guard[ Σ ]  τ  e").
-
-Notation "'static_guard[' Σ ']' τ" :=
-  (ty_static_guard_formula Σ τ)
-  (at level 20, Σ at level 200, τ at level 200,
-   format "static_guard[ Σ ]  τ").
-
-Notation "'static_guard[' Σ ']' τ e" :=
-  (ty_static_guard_formula Σ τ e)
-  (at level 20, Σ at level 200, τ at level 200, e at level 20,
-   format "static_guard[ Σ ]  τ  e").
-
 End TypeDenote.
+
+Notation "'TyDenote[' Δ ';' τ ';' e ']'" :=
+  (ty_denote Δ τ e)
+  (at level 20, Δ at level 200, τ at level 200, e at level 200,
+   format "TyDenote[ Δ ;  τ ;  e ]").
