CoreLang/theories/Sugar.v
@@ -46,17 +46,11 @@ Notation "e '·ₜ' v" := (tapp_tm e v)
   (at level 40, left associativity,
    format "e  ·ₜ  v").
 
-Notation "'↑{' k '}' v" := (value_shift k v)
-  (at level 20, k constr, only printing,
-   format "↑{ k }  v") : core_scope.
 Notation "'↑{' k '}' e" := (tm_shift k e)
-  (at level 20, k constr, only printing,
+  (at level 20, k constr,
    format "↑{ k }  e") : core_scope.
-Notation "v '↑'" := (value_shift 0 v)
-  (at level 20, only printing,
-   format "v  ↑") : core_scope.
 Notation "e '↑'" := (tm_shift 0 e)
-  (at level 20, only printing,
+  (at level 20,
    format "e  ↑") : core_scope.
 
 Lemma value_shift_fv k v :
